case_study/RiscvPmp/Contracts.v
@@ -1274,7 +1274,7 @@ Module Import RiscvPmpSpecification <: Specification RiscvPmpBase RiscvPmpSignat
 End RiscvPmpSpecification.
 
 Module RiscvPmpExecutor :=
-  MakeExecutor RiscvPmpBase RiscvPmpSignature RiscvPmpSolver RiscvPmpProgram RiscvPmpSpecification.
+  MakeExecutor RiscvPmpBase RiscvPmpSignature RiscvPmpProgram RiscvPmpSpecification.
 
 Module RiscvPmpShallowExecutor :=
   MakeShallowExecutor RiscvPmpBase RiscvPmpSignature RiscvPmpProgram RiscvPmpSpecification.
